---
title: "Clase 4_Ejemplos"
author: "Jhonatan Smith Garcia"
date: "13/10/2021"
output: pdf_document
---

```{r setup, include=FALSE}
knitr::opts_chunk$set(echo = TRUE)
```

$$

 E(Y-\widehat{Y})^{2}=E[f(x)+\varepsilon-\widehat{f}(x)]^{2}

=E[(f(x)+\varepsilon-\widehat{f}(x))(f(x)+\varepsilon-\widehat{f}(x))

=E[((f(x)-\widehat{f}(x))+\varepsilon )(f(x)+\varepsilon -\widehat{f}(x))]

=E[(f(x)-\widehat{f}(x))(f(x)+\varepsilon -\widehat{f}(x))+\varepsilon (f(x)+\varepsilon -\widehat{f}(x))]
$$
$$

=E[(f(x)-\widehat{f}(x))(f(x)-\widehat{f}(x)+\varepsilon) +\varepsilon (f(x)+\varepsilon -\widehat{f}(x))]

=E[((f(x)-\widehat{f}(x))^{2}]+\varepsilon(f(x)-\widehat{f}(x))+\varepsilon((f(x)-\widehat{f}(x))+\varepsilon)]=

$$

$$
E[((f(x)-\widehat{f}(x))^{2}+\varepsilon (f(x)-\widehat{f}(x))+\varepsilon (f(x)-\widehat{f}(x))+(\varepsilon ^{2})]=

E[((f(x)-\widehat{f}(x))^{2}]+2E[f(x)-\widehat{f}(x)]+E[(\varepsilon ^{2})]=

(f(x)-\widehat{f}(x))^{2}+0+var(\varepsilon )=(f(x)-\widehat{f}(x))^{2}+var(\varepsilon )

\newpage
$$